

Momentum Descent

{ heavy ball method }

Plain gradient descent: $\theta_{t+1} = \theta_t - \eta \nabla J(\theta_t)$

But has ① ill conditioned Hessians.

② Oscillate across steep directions.

③ Move slowly along flat directions.

Momentum fixes this by accumulating velocity, not just reaching to the current gradient.

Analogy: ① Gradient \rightarrow Force

② Momentum \rightarrow Velocity

③ Parameters \rightarrow Position

$$v^* \in \mathbb{R}^d$$

$\mu \rightarrow$ Momentum

(β) Coefficient (0.9)

$$F = m \frac{dv}{dt} \Rightarrow F dt = m dv$$

Momentum is exponentially weighted moving average of past gradients.

* Algebraic form

θ_0 given, $v_0 = 0$

* Update Rule

$$v_t = \mu v_{t-1} + g_t = \mu (\mu v_{t-2} + g_{t-1}) + g_t = \dots \sum_{k=0}^t \mu^k g_{t-k}$$

$$\theta_{t+1} = \theta_t - \eta v_t$$

$$v_t = \beta v_{t-1} + (1-\beta) \nabla_{\theta} J(\theta_t)$$

$$\theta_{t+1} = \theta_t - \eta v_t$$

* Example: $\{(1,2), (2,3), (3,5)\} \rightarrow$ Fitting linear regression with momentum GD.

\rightarrow model: $y = wx + b$ $\theta = \begin{pmatrix} w \\ b \end{pmatrix}$

$$\begin{aligned} \mathcal{L} &= J(\theta) = \frac{1}{2m} \sum_0^m (\hat{y}_i - y)^2 \\ &= \frac{1}{2m} (\hat{y} - y)^T (\hat{y} - y) \\ &= \frac{1}{2m} (x\theta - y)^T (x\theta - y) \\ &= \frac{1}{2m} (\theta^T x^T x \theta - x^T \theta^T y - y^T x \theta - y^T y) \\ &= \frac{1}{2m} (\theta^T x^T x \theta - 2x^T \theta^T y - y^T y) \end{aligned}$$

initialisations

$$\theta = \begin{pmatrix} 0 \\ 0 \end{pmatrix} \quad v = \begin{pmatrix} v_w \\ v_b \end{pmatrix} \in \mathbb{R}^2$$

$$\eta = 0.1$$

$$\beta = 0.9$$

$$x = \begin{pmatrix} 1 & 1 \\ 2 & 1 \\ 3 & 1 \end{pmatrix} \in \mathbb{R}^{3 \times 2}$$

$$y = \begin{pmatrix} 2 \\ 3 \\ 5 \end{pmatrix}$$

$$\hat{y} = x\theta$$

$$\nabla_{\theta} J(\theta) = \frac{1}{m} x^T (x\theta - y)$$

* Update rules:

$$v_t = \beta v_{t-1} + (1-\beta) \nabla J(\theta_t)$$

$$\theta_{t+1} = \theta_t - \eta v_t$$

* Predictions: $x\theta = \begin{pmatrix} 0 \\ 0 \\ 0 \end{pmatrix} = \hat{y}_0$ $e_0 = \begin{pmatrix} -2 \\ -3 \\ -5 \end{pmatrix}$

1st iteration

$$\nabla J(\theta) = \frac{1}{3} \begin{pmatrix} 1 & 2 & 3 \\ 1 & 1 & 1 \end{pmatrix} \begin{pmatrix} -2 \\ -3 \\ -5 \end{pmatrix} = \begin{pmatrix} -7.667 \\ -0.333 \end{pmatrix}$$

$$v_1 = (0.9) \begin{pmatrix} 0 \\ 0 \end{pmatrix} + (1-0.9) \begin{pmatrix} -7.667 \\ -0.333 \end{pmatrix} = \begin{pmatrix} -0.767 \\ -0.333 \end{pmatrix}$$

$$\theta_1 = \begin{pmatrix} 0 \\ 0 \end{pmatrix} - 0.1 \begin{pmatrix} 0.767 \\ 0.333 \end{pmatrix} = \begin{pmatrix} 0.0767 \\ 0.0333 \end{pmatrix}$$